add(Modal/Neighborhood): Supplementaion of Frame (#472)

Foundation/Modal/Neighborhood/AxiomC.lean
@@ -1,4 +1,5 @@
 import Foundation.Modal.Neighborhood.Basic
+import Foundation.Modal.Neighborhood.Completeness
 
 namespace LO.Modal.Neighborhood
 
@@ -7,9 +8,9 @@ open Formula.Neighborhood
 variable {F : Frame}
 
 class Frame.IsRegular (F : Frame) : Prop where
-  regular : ∀ X Y : Set F, (ℬ X) ∩ (ℬ Y) ⊆ ℬ (X ∩ Y)
+  regular : ∀ X Y, (F.box X) ∩ (F.box Y) ⊆ F.box (X ∩ Y)
 
-lemma Frame.regular [Frame.IsRegular F] {X Y : Set F} : (ℬ X) ∩ (ℬ Y) ⊆ ℬ (X ∩ Y) := by apply IsRegular.regular
+lemma Frame.regular [Frame.IsRegular F] {X Y : Set F} : (F.box X) ∩ (F.box Y) ⊆ F.box (X ∩ Y) := by apply IsRegular.regular
 
 instance : Frame.simple_blackhole.IsRegular := ⟨by
   intro X Y e;
@@ -29,5 +30,31 @@ lemma valid_axiomC_of_isRegular [F.IsRegular] : F ⊧ Axioms.C (.atom 0) (.atom 
   constructor;
   . apply h₁;
   . apply h₂;
+
+
+section
+
+variable [Entailment (Formula ℕ) S]
+variable {𝓢 : S} [Entailment.Consistent 𝓢] [Entailment.EC 𝓢]
+
+open Entailment
+open MaximalConsistentSet
+
+instance : (minimalCanonicalFrame 𝓢).IsRegular := by
+  constructor;
+  rintro X Y Γ ⟨hX, hY⟩;
+  obtain ⟨φ, rfl, hφ⟩ := minimalCanonicalFrame.exists_box X Γ hX;
+  obtain ⟨ψ, rfl, hψ⟩ := minimalCanonicalFrame.exists_box Y Γ hY;
+  rw [(show proofset 𝓢 φ ∩ proofset 𝓢 ψ = proofset 𝓢 (φ ⋏ ψ) by simp)];
+  have : proofset 𝓢 (□φ ⋏ □ψ) ⊆ proofset 𝓢 (□(φ ⋏ ψ)) := proofset.imp_subset |>.mp (by simp);
+  have : Γ ∈ proofset 𝓢 (□(φ ⋏ ψ)) := this $ by
+    simp only [proofset.eq_and, Set.mem_inter_iff];
+    constructor;
+    . apply hφ ▸ hX;
+    . apply hψ ▸ hY;
+  convert this;
+  convert Frame.IsCanonical.box_proofset (F := minimalCanonicalFrame 𝓢) (𝓢 := 𝓢) (φ ⋏ ψ);
+
+end
 
 end LO.Modal.Neighborhood
