Foundation/Modal/Neighborhood/Completeness.lean
@@ -1,5 +1,6 @@
 import Foundation.Modal.MaximalConsistentSet
 import Foundation.Modal.Neighborhood.Basic
+import Foundation.Modal.Entailment.EM
 
 namespace LO.Modal
 
@@ -72,6 +73,12 @@ lemma eq_boxed_of_eq [Entailment.E 𝓢] : ‖φ‖ = ‖ψ‖ → ‖□φ‖ =
   apply iff_subset.mpr;
   assumption;
 
+@[grind]
+lemma box_subset_of_subset [Entailment.EM 𝓢] : ‖φ‖ ⊆ ‖ψ‖ → ‖□φ‖ ⊆ ‖□ψ‖ := by
+  intro h;
+  apply imp_subset.mp;
+  exact Entailment.rm! $ imp_subset.mpr h;
+
 end MaximalConsistentSet.proofset
 
 end
@@ -86,43 +93,65 @@ open Formula.Neighborhood
 open MaximalConsistentSet
 
 variable {S} [Entailment (Formula ℕ) S]
-variable {𝓢 : S} [Entailment.Cl 𝓢] [Entailment.Consistent 𝓢]
+variable {𝓢 : S} -- [Entailment.Cl 𝓢] [Entailment.Consistent 𝓢]
 variable {φ ψ ξ : Formula ℕ}
 
-structure CanonicalBox (𝓢 : S) where
-  box : Set (MaximalConsistentSet 𝓢) → Set (MaximalConsistentSet 𝓢)
-  canonicity : ∀ φ, box (proofset 𝓢 φ) = proofset 𝓢 (□φ)
+class Frame.IsCanonical (F : Frame) (𝓢 : S) : Prop where
+  eq_world : F.World = MaximalConsistentSet 𝓢 := by rfl
+  box_proofset : ∀ φ, F.box (eq_world ▸ (proofset 𝓢 φ)) = eq_world ▸ (proofset 𝓢 (□φ))
 
-instance : CoeFun (CanonicalBox 𝓢) (fun _ => Set (MaximalConsistentSet 𝓢) → Set (MaximalConsistentSet 𝓢)) := ⟨CanonicalBox.box⟩
+namespace Frame.IsCanonical
 
-def mkCanonicalFrame
-  (𝓢 : S) [Entailment.Consistent 𝓢] [Entailment.Cl 𝓢]
-  (box : CanonicalBox 𝓢)
-  : Frame := Frame.mk_ℬ (MaximalConsistentSet 𝓢) box
+variable {F : Frame} [canonical : F.IsCanonical 𝓢]
 
-def mkCanonicalModel
-  (𝓢 : S) [Entailment.Consistent 𝓢] [Entailment.Cl 𝓢]
-  (box : CanonicalBox 𝓢)
-  : Model where
-  toFrame := mkCanonicalFrame 𝓢 box
-  Val a := proofset 𝓢 (.atom a)
+@[simp]
+lemma eq_empty : (canonical.eq_world ▸ (∅ : Set (MaximalConsistentSet 𝓢))) = ∅ := by
+  have := canonical.eq_world;
+  grind;
 
-@[simp] lemma mkCanonicalModel.eq_ℬ_self : (mkCanonicalModel 𝓢 box).box = box := by tauto;
+@[simp]
+lemma eq_union {X Y : Set (MaximalConsistentSet 𝓢)} : (canonical.eq_world ▸ (X ∪ Y)) = ((canonical.eq_world ▸ X) ∪ (canonical.eq_world ▸ Y)) := by
+  have := canonical.eq_world;
+  grind;
 
-lemma truthlemma : ↑(proofset 𝓢 φ) = ((mkCanonicalModel 𝓢 box).truthset φ) := by
+@[simp]
+lemma eq_comp {X : Set (MaximalConsistentSet 𝓢)} : (canonical.eq_world ▸ Xᶜ) = (canonical.eq_world ▸ X)ᶜ := by
+  haveI := canonical.eq_world;
+  grind;
+
+@[simp]
+lemma iff_mem {Γ : MaximalConsistentSet 𝓢} {X : Set _} : Γ ∈ X ↔ (canonical.eq_world ▸ Γ) ∈ (canonical.eq_world ▸ X) := by
+  have := canonical.eq_world;
+  grind;
+
+end Frame.IsCanonical
+
+
+def canonicalModel (F : Frame) (𝓢 : S) [canonical : F.IsCanonical 𝓢] : Model where
+  toFrame := F
+  Val a := canonical.eq_world ▸ proofset 𝓢 (.atom a)
+
+namespace canonicalModel
+
+variable {F : Frame} [canonical : F.IsCanonical 𝓢]
+
+@[simp] lemma eq_model_box : (canonicalModel F 𝓢).box = F.box := by tauto;
+
+end canonicalModel
+
+variable [Entailment.Cl 𝓢]
+         {F : Frame} [canonical : F.IsCanonical 𝓢]
+
+lemma truthlemma : canonical.eq_world ▸ (proofset 𝓢 φ) = ((canonicalModel F 𝓢).truthset φ) := by
   induction φ with
-  | hatom =>
-    simp [mkCanonicalModel]
-  | hfalsum =>
-    simp [mkCanonicalModel]
-  | himp φ ψ ihφ ihψ =>
-    simp_all [MaximalConsistentSet.proofset.eq_imp, ←ihφ, ←ihψ];
+  | hatom => simp [canonicalModel]
+  | hfalsum => simp [canonicalModel];
+  | himp φ ψ ihφ ihψ => simp_all [MaximalConsistentSet.proofset.eq_imp, ←ihφ, ←ihψ];
   | hbox φ ihφ =>
-    rw [Model.truthset.eq_box, ←ihφ, mkCanonicalModel.eq_ℬ_self, (@box.canonicity φ)];
+    rw [Model.truthset.eq_box, ←ihφ, ←(canonical.box_proofset φ)];
+    rfl;
 
-lemma complete_of_canonical_frame
-  (C : FrameClass) (box)
-  (hC : (mkCanonicalFrame 𝓢 box) ∈ C)
+lemma complete_of_canonical_frame (C : FrameClass) (F : Frame) [canonical : F.IsCanonical 𝓢] (hC : F ∈ C)
   : LO.Complete 𝓢 C := by
   constructor;
   intro φ;
@@ -131,24 +160,91 @@ lemma complete_of_canonical_frame
   have := FormulaSet.unprovable_iff_singleton_neg_consistent.mpr hφ;
   obtain ⟨Γ, hΓ⟩ := lindenbaum this;
   apply not_validOnFrameClass_of_exists_model_world;
-  use (mkCanonicalModel 𝓢 box), Γ;
+  use (canonicalModel F 𝓢), (canonical.eq_world ▸ Γ);
   constructor;
   . assumption;
   . simp only [Semantics.Realize, Satisfies, ←truthlemma];
-    suffices Γ ∈ (proofset 𝓢 (∼φ)) by simpa;
+    suffices Γ ∈ (proofset 𝓢 (∼φ)) by
+      apply canonical.iff_mem.not.mp;
+      simpa using this;
     apply hΓ;
     tauto;
 
+
+
+
 open Classical in
-def minimal_canonical_box (𝓢 : S) [Entailment.E 𝓢] : CanonicalBox 𝓢 where
-  box Γ := if h : ∃ φ, Γ = (proofset 𝓢 φ) then (proofset 𝓢 (□(h.choose))) else ∅
-  canonicity := by
+abbrev minimalCanonicalFrame (𝓢 : S) [Entailment.E 𝓢] [Entailment.Consistent 𝓢] : Frame := Frame.mk_ℬ
+  (MaximalConsistentSet 𝓢)
+  (λ X => if h : ∃ φ, X = (proofset 𝓢 φ) then (proofset 𝓢 (□(h.choose))) else ∅)
+
+namespace minimalCanonicalFrame
+
+variable {𝓢 : S} [Entailment.E 𝓢] [Entailment.Consistent 𝓢]
+
+instance : (minimalCanonicalFrame 𝓢).IsCanonical 𝓢 where
+  box_proofset := by
     intro φ;
+    dsimp [minimalCanonicalFrame, Frame.mk_ℬ, Frame.box];
     split;
     . rename_i h;
       apply proofset.eq_boxed_of_eq;
       apply h.choose_spec.symm;
     . tauto;
+
+lemma exists_box (X) (Γ : (minimalCanonicalFrame 𝓢).World) (hΓ : Γ ∈ Frame.box _ X)
+  : ∃ φ, X = proofset 𝓢 φ ∧ Frame.box _ X = proofset 𝓢 (□φ)
+  := by
+    simp [Frame.mk_ℬ, Frame.box] at hΓ;
+    split at hΓ;
+    . rename_i h;
+      obtain ⟨φ, hφ⟩ := h;
+      use φ;
+      constructor;
+      . assumption;
+      . convert Frame.IsCanonical.box_proofset (F := minimalCanonicalFrame 𝓢) (𝓢 := 𝓢) φ;
+    . contradiction;
+
+/-
+lemma exists_dia (X) (Γ : (CanonicalBox.minimal 𝓢).model.World) (hΓ : Γ ∈ Frame.box _ X)
+  : ∃ φ, X = proofset 𝓢 φ ∧ Frame.dia _ X = proofset 𝓢 (◇φ)
+  := by
+    obtain ⟨φ, hφ, hΓ⟩ := exists_box X Γ hΓ;
+    use φ;
+    constructor;
+    . assumption;
+    . ext Γ;
+      rw [(show ◇φ = ∼□(∼φ) by rfl)];
+      simp only [
+        CanonicalBox.minimal, CanonicalBox.model, CanonicalBox.frame, Frame.mk_ℬ,
+        Frame.dia, Frame.box, Set.mem_setOf_eq, Set.setOf_mem_eq, Set.mem_compl_iff,
+        proofset.eq_neg
+      ];
+      constructor;
+      . intro h;
+        split at h;
+        . rename_i h₂;
+          suffices proofset 𝓢 (□h₂.choose) = proofset 𝓢 (□(∼φ)) by rw [this] at h; simpa;
+          apply proofset.eq_boxed_of_eq;
+          rw [←h₂.choose_spec, hφ];
+          simp;
+        . exfalso;
+          rename_i h₂;
+          push_neg at h₂;
+          apply @h₂ (∼φ);
+          simpa;
+      . intro h;
+        split;
+        . rename_i h₂;
+          suffices proofset 𝓢 (□h₂.choose) = proofset 𝓢 (□(∼φ)) by rw [←this] at h; simpa;
+          apply proofset.eq_boxed_of_eq;
+          rw [←h₂.choose_spec, hφ];
+          simp;
+        . tauto;
+-/
+
+end minimalCanonicalFrame
+
 
 end Neighborhood
 
