Foundation/Modal/Neighborhood/Supplementation.lean
@@ -1,0 +1,140 @@
+import Foundation.Modal.Neighborhood.Basic
+import Foundation.Modal.Neighborhood.AxiomM
+import Foundation.Modal.Neighborhood.AxiomC
+import Foundation.Modal.Neighborhood.AxiomGeach
+
+namespace LO.Modal.Neighborhood
+
+variable {F : Frame}
+
+def Frame.Supplementation (F : Frame) : Frame := Frame.mk_ℬ F.World (λ X => (Set.sUnion { F.box Y | Y ⊆ X }))
+
+local postfix:80 "♯" => Frame.Supplementation
+
+namespace Frame.Supplementation
+
+lemma iff_exists_subset {X : Set (F.World)} {w : F.World} : w ∈ F♯.box X ↔ ∃ Y ⊆ X, w ∈ F.box Y := by
+  simp [Frame.Supplementation, Frame.box, Frame.mk_ℬ, Set.mem_sUnion, Set.mem_setOf_eq, exists_exists_and_eq_and]
+
+lemma subset (X : Set (F.World)) : F.box X ⊆ F♯.box X := by
+  intro x;
+  simp [Frame.Supplementation, Frame.box, Frame.mk_ℬ];
+  tauto;
+
+lemma monotonic {X Y : Set (F.World)} (h : X ⊆ Y) : F♯.box X ⊆ F♯.box Y := by
+  intro x hX;
+  obtain ⟨X', hX', hX⟩ := iff_exists_subset.mp hX;
+  apply iff_exists_subset.mpr;
+  use X';
+  constructor;
+  . apply Set.Subset.trans hX' h;
+  . assumption;
+
+lemma monotonic_iterated {X Y : Set (F.World)} (h : X ⊆ Y) (n) : F♯.box^[n] X ⊆ F♯.box^[n] Y := by
+  induction n with
+  | zero => simpa;
+  | succ n ih =>
+    rw [Function.iterate_succ'];
+    apply monotonic;
+    apply ih;
+
+lemma itl_reduce : F♯♯.box X = F♯.box X := by
+  ext x;
+  simp only [Supplementation, mk_ℬ, Set.mem_setOf_eq, Set.mem_sUnion, exists_exists_and_eq_and]
+  constructor;
+  . rintro ⟨Y, RYX, Z, RZY, hZ⟩;
+    use Z;
+    constructor;
+    . tauto_set;
+    . assumption;
+  . tauto;
+
+instance : F♯.IsMonotonic := by
+  constructor;
+  rintro X Y x hx;
+  obtain ⟨W, hW₁, hW₂⟩ := iff_exists_subset.mp hx;
+  constructor <;>
+  . apply iff_exists_subset.mpr;
+    use W;
+    constructor;
+    . tauto_set;
+    . assumption;
+
+instance [F.IsReflexive] : F♯.IsReflexive := by
+  constructor;
+  intro X w hw;
+  replace ⟨Y, hY₁, hY₂⟩ := iff_exists_subset.mp hw;
+  apply hY₁;
+  apply F.refl;
+  exact hY₂;
+
+instance [F.IsTransitive] : F♯.IsTransitive := by
+  constructor;
+  intro X w hw;
+  obtain ⟨Y, hYX, hY⟩ := iff_exists_subset.mp hw;
+  apply monotonic_iterated hYX 2
+  apply monotonic $ subset Y;
+  apply subset (F.box Y) $ F.trans hY;
+
+instance [F.IsRegular] : F♯.IsRegular := by
+  constructor;
+  rintro X Y w ⟨hX, hY⟩;
+  apply iff_exists_subset.mpr;
+  obtain ⟨X', _⟩ := iff_exists_subset.mp hX;
+  obtain ⟨Y', _⟩ := iff_exists_subset.mp hY;
+  use X' ∩ Y';
+  constructor;
+  . tauto_set;
+  . apply @Frame.regular F _ X' Y';
+    tauto;
+
+end Frame.Supplementation
+
+
+section
+
+open MaximalConsistentSet (proofset)
+open MaximalConsistentSet.proofset
+
+variable {S} [Entailment (Formula ℕ) S]
+variable {𝓢 : S} [Entailment.Consistent 𝓢]
+
+abbrev supplementalMinimalCanonicalFrame (𝓢 : S) [Entailment.E 𝓢] [Entailment.Consistent 𝓢] : Frame := (minimalCanonicalFrame 𝓢)♯
+
+variable [Entailment.EM 𝓢]
+
+instance : (supplementalMinimalCanonicalFrame 𝓢).IsCanonical 𝓢 where
+  box_proofset := by
+    intro φ;
+    apply Set.eq_of_subset_of_subset;
+    . intro Γ;
+      simp only [
+        Frame.Supplementation, Frame.mk_ℬ, Set.mem_setOf_eq, Set.mem_sUnion,
+        exists_exists_and_eq_and, forall_exists_index, and_imp
+      ];
+      intro X hX h;
+      split at h;
+      . rename_i hψ;
+        rw [hψ.choose_spec] at hX;
+        apply box_subset_of_subset hX;
+        apply h;
+      . contradiction;
+    . intro Γ;
+      simp only [
+        Frame.Supplementation, Frame.mk_ℬ, Set.mem_setOf_eq, Set.mem_sUnion,
+        exists_exists_and_eq_and
+      ];
+      intro hΓ;
+      use proofset 𝓢 φ;
+      constructor
+      . rfl;
+      . split;
+        . rename_i hψ;
+          rw [←eq_boxed_of_eq hψ.choose_spec];
+          apply hΓ;
+        . simp_all;
+
+end
+
+
+end LO.Modal.Neighborhood
